coq/LambdaNRA/LambdaNRA.v
@@ -28,204 +28,204 @@ Section LambdaNRA.
   Unset Elimination Schemes.
 
   (* Lambda NRA *)
-  Inductive lalg : Set :=
-  | LAVar : string -> lalg (* Variable access *)
-  | LATable : string -> lalg
-  | LAConst : data -> lalg
-  | LABinop : binOp -> lalg -> lalg -> lalg
-  | LAUnop : unaryOp -> lalg -> lalg
-  | LAMap : lalg_lambda -> lalg -> lalg (* 'dependent operators' use lambdas *)
-  | LAMapConcat : lalg_lambda -> lalg -> lalg
-  | LAProduct : lalg -> lalg -> lalg
-  | LASelect : lalg_lambda -> lalg -> lalg
-  with lalg_lambda : Set :=
-  | LALambda : string -> lalg -> lalg_lambda (* Lambda is (\var.alg) *)
+  Inductive lnra : Set :=
+  | LNRAVar : string -> lnra (* Variable access *)
+  | LNRATable : string -> lnra
+  | LNRAConst : data -> lnra
+  | LNRABinop : binOp -> lnra -> lnra -> lnra
+  | LNRAUnop : unaryOp -> lnra -> lnra
+  | LNRAMap : lnra_lambda -> lnra -> lnra (* 'dependent operators' use lambdas *)
+  | LNRAMapConcat : lnra_lambda -> lnra -> lnra
+  | LNRAProduct : lnra -> lnra -> lnra
+  | LNRAFilter : lnra_lambda -> lnra -> lnra
+  with lnra_lambda : Set :=
+  | LNRALambda : string -> lnra -> lnra_lambda (* Lambda is (\var.alg) *)
   .
 
-  Tactic Notation "lalg_cases" tactic(first) ident(c) :=
+  Tactic Notation "lnra_cases" tactic(first) ident(c) :=
   first;
-  [ Case_aux c "LAVar"%string
-  | Case_aux c "LATable"%string
-  | Case_aux c "LAConst"%string
-  | Case_aux c "LABinop"%string
-  | Case_aux c "LAUnop"%string
-  | Case_aux c "LAMap"%string
-  | Case_aux c "LAMapConcat"%string
-  | Case_aux c "LAProduct"%string
-  | Case_aux c "LASelect"%string
+  [ Case_aux c "LNRAVar"%string
+  | Case_aux c "LNRATable"%string
+  | Case_aux c "LNRAConst"%string
+  | Case_aux c "LNRABinop"%string
+  | Case_aux c "LNRAUnop"%string
+  | Case_aux c "LNRAMap"%string
+  | Case_aux c "LNRAMapConcat"%string
+  | Case_aux c "LNRAProduct"%string
+  | Case_aux c "LNRAFilter"%string
   ].
   
   Set Elimination Schemes.
 
   (* The language is defined via mutual recursion, but it is easier to 
      unfold it for reasoning. *)
-  Definition  lalg_rect
-              (P : lalg -> Type)
-              (fvar : forall s : string, P (LAVar s))
-              (ftable : forall t : string, P (LATable t))
-              (fconst : forall d : data, P (LAConst d))
-              (fbinop : forall (b : binOp) (l : lalg), P l -> forall l0 : lalg, P l0 -> P (LABinop b l l0))
-              (funop : forall (u : unaryOp) (l : lalg), P l -> P (LAUnop u l))
-              (fmap : forall (s:string) (l0 l1 : lalg), P l0 -> P l1 -> P (LAMap (LALambda s l0) l1))
-              (fmapconcat : forall (s:string) (l0 l1 : lalg), P l0 -> P l1 -> P (LAMapConcat (LALambda s l0) l1))
-              (fproduct : forall l : lalg, P l -> forall l0 : lalg, P l0 -> P (LAProduct l l0))
-              (fselect : forall (s:string) (l0 l1 : lalg), P l0 -> P l1 -> P (LASelect (LALambda s l0) l1)) :
+  Definition  lnra_rect
+              (P : lnra -> Type)
+              (fvar : forall s : string, P (LNRAVar s))
+              (ftable : forall t : string, P (LNRATable t))
+              (fconst : forall d : data, P (LNRAConst d))
+              (fbinop : forall (b : binOp) (l : lnra), P l -> forall l0 : lnra, P l0 -> P (LNRABinop b l l0))
+              (funop : forall (u : unaryOp) (l : lnra), P l -> P (LNRAUnop u l))
+              (fmap : forall (s:string) (l0 l1 : lnra), P l0 -> P l1 -> P (LNRAMap (LNRALambda s l0) l1))
+              (fmapconcat : forall (s:string) (l0 l1 : lnra), P l0 -> P l1 -> P (LNRAMapConcat (LNRALambda s l0) l1))
+              (fproduct : forall l : lnra, P l -> forall l0 : lnra, P l0 -> P (LNRAProduct l l0))
+              (ffilter : forall (s:string) (l0 l1 : lnra), P l0 -> P l1 -> P (LNRAFilter (LNRALambda s l0) l1)) :
     forall l, P l
     := 
-      fix F (l : lalg) : P l :=
+      fix F (l : lnra) : P l :=
         match l as l0 return (P l0) with
-        | LAVar s => fvar s
-        | LATable t => ftable t
-        | LAConst d => fconst d
-        | LABinop b l0 l1 => fbinop b l0 (F l0) l1 (F l1)
-        | LAUnop u l0 => funop u l0 (F l0)
-        | LAMap (LALambda s l0) l1 => fmap s l0 l1 (F l0) (F l1)
-        | LAMapConcat (LALambda s l0) l1 => fmapconcat s l0 l1 (F l0) (F l1)
-        | LAProduct l0 l1 => fproduct l0 (F l0) l1 (F l1)
-        | LASelect (LALambda s l0) l1 => fselect s l0 l1 (F l0) (F l1)
+        | LNRAVar s => fvar s
+        | LNRATable t => ftable t
+        | LNRAConst d => fconst d
+        | LNRABinop b l0 l1 => fbinop b l0 (F l0) l1 (F l1)
+        | LNRAUnop u l0 => funop u l0 (F l0)
+        | LNRAMap (LNRALambda s l0) l1 => fmap s l0 l1 (F l0) (F l1)
+        | LNRAMapConcat (LNRALambda s l0) l1 => fmapconcat s l0 l1 (F l0) (F l1)
+        | LNRAProduct l0 l1 => fproduct l0 (F l0) l1 (F l1)
+        | LNRAFilter (LNRALambda s l0) l1 => ffilter s l0 l1 (F l0) (F l1)
         end.
 
-  Definition lalg_ind (P : lalg -> Prop) := lalg_rect P.
-  Definition lalg_rec (P:lalg->Set) := lalg_rect P.
+  Definition lnra_ind (P : lnra -> Prop) := lnra_rect P.
+  Definition lnra_rec (P:lnra->Set) := lnra_rect P.
 
   (** Semantics of Lambda NRA *)
 
   Context (h:brand_relation_t).
   Context (constant_env:list (string*data)).
 
-  Fixpoint fun_of_lalg (env: bindings) (op:lalg) : option data :=
+  Fixpoint fun_of_lnra (env: bindings) (op:lnra) : option data :=
     match op with
-    | LAVar x => edot env x
-    | LATable t => edot constant_env t
-    | LAConst d => Some (normalize_data h d)
-    | LABinop b op1 op2 => olift2 (fun d1 d2 => fun_of_binop h b d1 d2) (fun_of_lalg env op1) (fun_of_lalg env op2)
-    | LAUnop u op1 =>
-      olift (fun d1 => fun_of_unaryop h u d1) (fun_of_lalg env op1)
-    | LAMap lop1 op2 =>
+    | LNRAVar x => edot env x
+    | LNRATable t => edot constant_env t
+    | LNRAConst d => Some (normalize_data h d)
+    | LNRABinop b op1 op2 => olift2 (fun d1 d2 => fun_of_binop h b d1 d2) (fun_of_lnra env op1) (fun_of_lnra env op2)
+    | LNRAUnop u op1 =>
+      olift (fun d1 => fun_of_unaryop h u d1) (fun_of_lnra env op1)
+    | LNRAMap lop1 op2 =>
         let aux_map d :=
-            lift_oncoll (fun c1 => lift dcoll (rmap (fun_of_lalg_lambda env lop1) c1)) d
-        in olift aux_map (fun_of_lalg env op2)
-    | LAMapConcat lop1 op2 =>
+            lift_oncoll (fun c1 => lift dcoll (rmap (fun_of_lnra_lambda env lop1) c1)) d
+        in olift aux_map (fun_of_lnra env op2)
+    | LNRAMapConcat lop1 op2 =>
       let aux_mapconcat d :=
-          lift_oncoll (fun c1 => lift dcoll (rmap_concat (fun_of_lalg_lambda env lop1) c1)) d
-      in olift aux_mapconcat (fun_of_lalg env op2)
-    | LAProduct op1 op2 =>
+          lift_oncoll (fun c1 => lift dcoll (rmap_concat (fun_of_lnra_lambda env lop1) c1)) d
+      in olift aux_mapconcat (fun_of_lnra env op2)
+    | LNRAProduct op1 op2 =>
       (* Note: it's even clearer from this formulation that both branches take the same environment *)
       let aux_product d :=
-          lift_oncoll (fun c1 => lift dcoll (rmap_concat (fun _ => fun_of_lalg env op2) c1)) d
-      in olift aux_product (fun_of_lalg env op1)
-    | LASelect lop1 op2 =>
+          lift_oncoll (fun c1 => lift dcoll (rmap_concat (fun _ => fun_of_lnra env op2) c1)) d
+      in olift aux_product (fun_of_lnra env op1)
+    | LNRAFilter lop1 op2 =>
       let pred x' :=
-          match fun_of_lalg_lambda env lop1 x' with
+          match fun_of_lnra_lambda env lop1 x' with
           | Some (dbool b) => Some b
           | _ => None
           end
       in
-      let aux_select d :=
+      let aux_map d :=
           lift_oncoll (fun c1 => lift dcoll (lift_filter pred c1)) d
       in
-      olift aux_select (fun_of_lalg env op2)
+      olift aux_map (fun_of_lnra env op2)
     end
-  with fun_of_lalg_lambda (env:bindings) (lop:lalg_lambda) (d:data) : option data :=
+  with fun_of_lnra_lambda (env:bindings) (lop:lnra_lambda) (d:data) : option data :=
     match lop with
-    | LALambda x op =>
-      (fun_of_lalg (env++((x,d)::nil)) op)
+    | LNRALambda x op =>
+      (fun_of_lnra (env++((x,d)::nil)) op)
     end.
 
   (* For top-level: Parametric query *)
-  Definition q_to_lambda (Q:lalg -> lalg) :=
-    (LALambda "input" (Q (LAVar "input"))).
+  Definition q_to_lambda (Q:lnra -> lnra) :=
+    (LNRALambda "input" (Q (LNRAVar "input"))).
 
-  Definition eval_q (Q:lalg -> lalg) (input:data) : option data :=
-    fun_of_lalg_lambda nil (q_to_lambda Q) input.
+  Definition eval_q (Q:lnra -> lnra) (input:data) : option data :=
+    fun_of_lnra_lambda nil (q_to_lambda Q) input.
 
 
-  Lemma fun_of_lalg_lambda_lambda_eq env x lop d:
-    fun_of_lalg_lambda env (LALambda x lop) d =
-    (fun_of_lalg (env++((x,d)::nil)) lop).
+  Lemma fun_of_lnra_lambda_lambda_eq env x lop d:
+    fun_of_lnra_lambda env (LNRALambda x lop) d =
+    (fun_of_lnra (env++((x,d)::nil)) lop).
   Proof.
     reflexivity.
   Qed.
 
-  Lemma fun_of_lalg_map_eq env lop1 op2 :
-    fun_of_lalg env (LAMap lop1 op2) = 
+  Lemma fun_of_lnra_map_eq env lop1 op2 :
+    fun_of_lnra env (LNRAMap lop1 op2) = 
         let aux_map d :=
-            lift_oncoll (fun c1 => lift dcoll (rmap (fun_of_lalg_lambda env lop1) c1)) d
-        in olift aux_map (fun_of_lalg env op2).
+            lift_oncoll (fun c1 => lift dcoll (rmap (fun_of_lnra_lambda env lop1) c1)) d
+        in olift aux_map (fun_of_lnra env op2).
   Proof.
     reflexivity.
   Qed.
 
-  Lemma fun_of_lalg_map_concat_eq env lop1 op2 :
-    fun_of_lalg env (LAMapConcat lop1 op2) = 
+  Lemma fun_of_lnra_map_concat_eq env lop1 op2 :
+    fun_of_lnra env (LNRAMapConcat lop1 op2) = 
       let aux_mapconcat d :=
-          lift_oncoll (fun c1 => lift dcoll (rmap_concat (fun_of_lalg_lambda env lop1) c1)) d
-      in olift aux_mapconcat (fun_of_lalg env op2).
+          lift_oncoll (fun c1 => lift dcoll (rmap_concat (fun_of_lnra_lambda env lop1) c1)) d
+      in olift aux_mapconcat (fun_of_lnra env op2).
   Proof.
     reflexivity.
   Qed.
 
-  Lemma fun_of_lalg_product_eq env op1 op2 :
-    fun_of_lalg env (LAProduct op1 op2) = 
+  Lemma fun_of_lnra_product_eq env op1 op2 :
+    fun_of_lnra env (LNRAProduct op1 op2) = 
         let aux_product d :=
-          lift_oncoll (fun c1 => lift dcoll (rmap_concat (fun _ => fun_of_lalg env op2) c1)) d
-        in olift aux_product (fun_of_lalg env op1).
+          lift_oncoll (fun c1 => lift dcoll (rmap_concat (fun _ => fun_of_lnra env op2) c1)) d
+        in olift aux_product (fun_of_lnra env op1).
   Proof.
     reflexivity.
   Qed.
 
-  Lemma fun_of_lalg_select_eq env lop1 op2 :
-    fun_of_lalg env (LASelect lop1 op2) = 
+  Lemma fun_of_lnra_filter_eq env lop1 op2 :
+    fun_of_lnra env (LNRAFilter lop1 op2) = 
       let pred x' :=
-          match fun_of_lalg_lambda env lop1 x' with
+          match fun_of_lnra_lambda env lop1 x' with
           | Some (dbool b) => Some b
           | _ => None
           end
       in
-      let aux_select d :=
+      let aux_map d :=
           lift_oncoll (fun c1 => lift dcoll (lift_filter pred c1)) d
       in
-      olift aux_select (fun_of_lalg env op2).
+      olift aux_map (fun_of_lnra env op2).
   Proof.
     reflexivity.
   Qed.
 
-  Lemma fun_of_lalg_normalized {op:lalg} {env:bindings} {o} :
-    fun_of_lalg env op= Some o ->
+  Lemma fun_of_lnra_normalized {op:lnra} {env:bindings} {o} :
+    fun_of_lnra env op= Some o ->
     Forall (fun x => data_normalized h (snd x)) env ->
     Forall (fun x => data_normalized h (snd x)) constant_env ->
     data_normalized h o.
   Proof.
     revert env o.
-    lalg_cases (induction op) Case
+    lnra_cases (induction op) Case
     ; intros; simpl in *.
-    - Case "LAVar"%string.
+    - Case "LNRAVar"%string.
       unfold edot in H.
       apply assoc_lookupr_in in H.
       rewrite Forall_forall in H0.
       specialize (H0 _ H).
       simpl in H0.
       trivial.
-    - Case "LATable"%string.
+    - Case "LNRATable"%string.
       unfold edot in H.
       apply assoc_lookupr_in in H.
       rewrite Forall_forall in H1.
       specialize (H1 _ H).
       simpl in H1.
       trivial.
-    - Case "LAConst"%string.
+    - Case "LNRAConst"%string.
       invcs H.
       apply normalize_normalizes.
-    - Case "LABinop"%string.
+    - Case "LNRABinop"%string.
       unfold olift2 in H.
       match_case_in H; intros; rewrite H2 in H; try discriminate.
       match_case_in H; intros; rewrite H3 in H; try discriminate.
       eapply fun_of_binop_normalized; eauto.
-    - Case "LAUnop"%string.
+    - Case "LNRAUnop"%string.
       unfold olift in H.
       match_case_in H; intros; rewrite H2 in H; try discriminate.
       eapply fun_of_unaryop_normalized; eauto.
-    - Case "LAMap"%string.
+    - Case "LNRAMap"%string.
       unfold olift in H.
       match_case_in H; intros; rewrite H2 in H; try discriminate.
       specialize (IHop2 _ _ H2 H0 H1).
@@ -239,7 +239,7 @@ Section LambdaNRA.
       + apply H3.
       + intros. eapply IHop1; eauto.
         apply Forall_app; auto.
-    - Case "LAMapConcat"%string.
+    - Case "LNRAMapConcat"%string.
       unfold olift in H.
       match_case_in H; intros; rewrite H2 in H; try discriminate.
       specialize (IHop2 _ _ H2 H0 H1).
@@ -278,7 +278,7 @@ Section LambdaNRA.
         apply Forall_app; trivial.
         constructor; trivial.
         trivial.
-    - Case "LAProduct"%string.
+    - Case "LNRAProduct"%string.
       unfold olift in H.
       match_case_in H; intros; rewrite H2 in H; try discriminate.
       specialize (IHop1 _ _ H2 H0 H1).
@@ -316,7 +316,7 @@ Section LambdaNRA.
         }
         trivial.
         trivial.
-    - Case "LASelect"%string.
+    - Case "LNRAFilter"%string.
       unfold olift in H.
       match_case_in H; intros; rewrite H2 in H; try discriminate.
       specialize (IHop2 _ _ H2 H0 H1).
@@ -333,69 +333,69 @@ Section LambdaNRA.
   
   Section LambdaNRAScope.
 
-    Fixpoint lalg_free_vars (e:lalg) :=
+    Fixpoint lnra_free_vars (e:lnra) :=
       match e with
-      | LAConst d => nil
-      | LAVar v => v :: nil
-      | LATable t => nil
-      | LABinop bop e1 e2 => lalg_free_vars e1 ++ lalg_free_vars e2
-      | LAUnop uop e1 => lalg_free_vars e1
-      | LAMap (LALambda x e1) e2 =>
-        (remove string_eqdec x (lalg_free_vars e1)) ++ (lalg_free_vars e2)
-      | LAMapConcat (LALambda x e1) e2 =>
-        (remove string_eqdec x (lalg_free_vars e1)) ++ (lalg_free_vars e2)
-      | LAProduct e1 e2 =>
-        (lalg_free_vars e1) ++ (lalg_free_vars e2)
-      | LASelect (LALambda x e1) e2 =>
-        (remove string_eqdec x (lalg_free_vars e1)) ++ (lalg_free_vars e2)
+      | LNRAConst d => nil
+      | LNRAVar v => v :: nil
+      | LNRATable t => nil
+      | LNRABinop bop e1 e2 => lnra_free_vars e1 ++ lnra_free_vars e2
+      | LNRAUnop uop e1 => lnra_free_vars e1
+      | LNRAMap (LNRALambda x e1) e2 =>
+        (remove string_eqdec x (lnra_free_vars e1)) ++ (lnra_free_vars e2)
+      | LNRAMapConcat (LNRALambda x e1) e2 =>
+        (remove string_eqdec x (lnra_free_vars e1)) ++ (lnra_free_vars e2)
+      | LNRAProduct e1 e2 =>
+        (lnra_free_vars e1) ++ (lnra_free_vars e2)
+      | LNRAFilter (LNRALambda x e1) e2 =>
+        (remove string_eqdec x (lnra_free_vars e1)) ++ (lnra_free_vars e2)
       end.
 
   (* capture avoiding substitution *)
-    Fixpoint lalg_subst (e:lalg) (x:string) (e':lalg) : lalg :=
+    Fixpoint lnra_subst (e:lnra) (x:string) (e':lnra) : lnra :=
       match e with
-      | LAConst d => LAConst d
-      | LAVar y => if y == x then e' else LAVar y
-      | LATable t => LATable t
-      | LABinop bop e1 e2 => LABinop bop
-                                   (lalg_subst e1 x e') 
-                                   (lalg_subst e2 x e')
-      | LAUnop uop e1 => LAUnop uop (lalg_subst e1 x e')
-      | LAMap (LALambda y e1) e2 =>
+      | LNRAConst d => LNRAConst d
+      | LNRAVar y => if y == x then e' else LNRAVar y
+      | LNRATable t => LNRATable t
+      | LNRABinop bop e1 e2 => LNRABinop bop
+                                   (lnra_subst e1 x e') 
+                                   (lnra_subst e2 x e')
+      | LNRAUnop uop e1 => LNRAUnop uop (lnra_subst e1 x e')
+      | LNRAMap (LNRALambda y e1) e2 =>
         if (y == x)
-        then LAMap (LALambda y e1) (lalg_subst e2 x e')
-        else LAMap (LALambda y (lalg_subst e1 x e')) (lalg_subst e2 x e')
-      | LAMapConcat (LALambda y e1) e2 =>
+        then LNRAMap (LNRALambda y e1) (lnra_subst e2 x e')
+        else LNRAMap (LNRALambda y (lnra_subst e1 x e')) (lnra_subst e2 x e')
+      | LNRAMapConcat (LNRALambda y e1) e2 =>
         if (y == x)
-        then LAMapConcat (LALambda y e1) (lalg_subst e2 x e')
-        else LAMapConcat (LALambda y (lalg_subst e1 x e')) (lalg_subst e2 x e')
-      | LAProduct e1 e2 =>
-        LAProduct (lalg_subst e1 x e') (lalg_subst e2 x e')
-      | LASelect (LALambda y e1) e2 =>
+        then LNRAMapConcat (LNRALambda y e1) (lnra_subst e2 x e')
+        else LNRAMapConcat (LNRALambda y (lnra_subst e1 x e')) (lnra_subst e2 x e')
+      | LNRAProduct e1 e2 =>
+        LNRAProduct (lnra_subst e1 x e') (lnra_subst e2 x e')
+      | LNRAFilter (LNRALambda y e1) e2 =>
         if (y == x)
-        then LASelect (LALambda y e1) (lalg_subst e2 x e')
-        else LASelect (LALambda y (lalg_subst e1 x e')) (lalg_subst e2 x e')
+        then LNRAFilter (LNRALambda y e1) (lnra_subst e2 x e')
+        else LNRAFilter (LNRALambda y (lnra_subst e1 x e')) (lnra_subst e2 x e')
       end.
 
   End LambdaNRAScope.
 End LambdaNRA.
 
-Hint Rewrite @fun_of_lalg_lambda_lambda_eq : lalg.
-Hint Rewrite @fun_of_lalg_map_eq : lalg.
-Hint Rewrite @fun_of_lalg_map_concat_eq : lalg.
-Hint Rewrite @fun_of_lalg_product_eq : lalg.
-Hint Rewrite @fun_of_lalg_select_eq : lalg.
+Hint Rewrite @fun_of_lnra_lambda_lambda_eq : lnra.
+Hint Rewrite @fun_of_lnra_map_eq : lnra.
+Hint Rewrite @fun_of_lnra_map_concat_eq : lnra.
+Hint Rewrite @fun_of_lnra_product_eq : lnra.
+Hint Rewrite @fun_of_lnra_filter_eq : lnra.
 
-Tactic Notation "lalg_cases" tactic(first) ident(c) :=
+Tactic Notation "lnra_cases" tactic(first) ident(c) :=
   first;
-  [ Case_aux c "LAVar"%string
-  | Case_aux c "LATable"%string
-  | Case_aux c "LAConst"%string
-  | Case_aux c "LABinop"%string
-  | Case_aux c "LAUnop"%string
-  | Case_aux c "LAMap"%string
-  | Case_aux c "LAMapConcat"%string
-  | Case_aux c "LAProduct"%string
-  | Case_aux c "LASelect"%string
+  [ Case_aux c "LNRAVar"%string
+  | Case_aux c "LNRATable"%string
+  | Case_aux c "LNRAConst"%string
+  | Case_aux c "LNRABinop"%string
+  | Case_aux c "LNRAUnop"%string
+  | Case_aux c "LNRAMap"%string
+  | Case_aux c "LNRAMapConcat"%string
+  | Case_aux c "LNRAProduct"%string
+  | Case_aux c "LNRAFilter"%string
   ].
 
 (* 
