coq/LambdaNRA/LambdaNRAEq.v
@@ -27,16 +27,16 @@ Section LambdaNRAEq.
 
   Context {fruntime:foreign_runtime}.
 
-    Definition lalg_eq (op1 op2:lalg) : Prop :=
+    Definition lnra_eq (op1 op2:lnra) : Prop :=
     forall
       (h:list(string*string))
       (cenv:bindings)
       (env:bindings)
       (dn_cenv:Forall (fun d => data_normalized h (snd d)) cenv)
       (dn_env:Forall (fun d => data_normalized h (snd d)) env),
-       fun_of_lalg h cenv env op1 = fun_of_lalg h cenv env op2.
+       fun_of_lnra h cenv env op1 = fun_of_lnra h cenv env op2.
 
-    Definition lalg_lambda_eq (op1 op2:lalg_lambda) : Prop :=
+    Definition lnra_lambda_eq (op1 op2:lnra_lambda) : Prop :=
     forall
       (h:list(string*string))
       (cenv:bindings)
@@ -45,55 +45,55 @@ Section LambdaNRAEq.
       (dn_env:Forall (fun d => data_normalized h (snd d)) env)
       (d:data)
       (dn_d:data_normalized h d),
-      fun_of_lalg_lambda h cenv env op1 d = fun_of_lalg_lambda h cenv env op2 d.
+      fun_of_lnra_lambda h cenv env op1 d = fun_of_lnra_lambda h cenv env op2 d.
 
-  Global Instance lalg_equiv : Equivalence lalg_eq.
+  Global Instance lnra_equiv : Equivalence lnra_eq.
   Proof.
     constructor.
-    - unfold Reflexive, lalg_eq.
+    - unfold Reflexive, lnra_eq.
       intros; reflexivity.
-    - unfold Symmetric, lalg_eq.
+    - unfold Symmetric, lnra_eq.
       intros. rewrite (H h cenv env dn_cenv dn_env) by trivial; reflexivity.
-    - unfold Transitive, lalg_eq.
+    - unfold Transitive, lnra_eq.
       intros. rewrite (H h cenv env dn_cenv dn_env) by trivial; rewrite (H0 h cenv env dn_cenv dn_env) by trivial; reflexivity.
   Qed.
 
-  Global Instance lalg_lambda_equiv : Equivalence lalg_lambda_eq.
+  Global Instance lnra_lambda_equiv : Equivalence lnra_lambda_eq.
   Proof.
     constructor.
-    - unfold Reflexive, lalg_lambda_eq.
+    - unfold Reflexive, lnra_lambda_eq.
       intros; reflexivity.
-    - unfold Symmetric, lalg_lambda_eq.
+    - unfold Symmetric, lnra_lambda_eq.
       intros. rewrite (H h cenv env dn_cenv dn_env) by trivial; reflexivity.
-    - unfold Transitive, lalg_lambda_eq.
+    - unfold Transitive, lnra_lambda_eq.
       intros. rewrite (H h cenv env dn_cenv dn_env) by trivial; rewrite (H0 h cenv env dn_cenv dn_env) by trivial; reflexivity.
   Qed.
 
-  Global Instance lavar_proper : Proper (eq ==> lalg_eq) LAVar.
+  Global Instance lavar_proper : Proper (eq ==> lnra_eq) LNRAVar.
   Proof.
-    unfold Proper, respectful, lalg_eq; intros.
+    unfold Proper, respectful, lnra_eq; intros.
     subst.
     reflexivity.
   Qed.
 
-  Global Instance latable_proper : Proper (eq ==> lalg_eq) LATable.
+  Global Instance latable_proper : Proper (eq ==> lnra_eq) LNRATable.
   Proof.
-    unfold Proper, respectful, lalg_eq; intros.
+    unfold Proper, respectful, lnra_eq; intros.
     subst.
     reflexivity.
   Qed.
 
-  Global Instance laconst_proper : Proper (eq ==> lalg_eq) LAConst.
+  Global Instance laconst_proper : Proper (eq ==> lnra_eq) LNRAConst.
   Proof.
-    unfold Proper, respectful, lalg_eq; intros.
+    unfold Proper, respectful, lnra_eq; intros.
     subst.
     reflexivity.
   Qed.
 
   Global Instance labinop_proper :
-    Proper (eq ==> lalg_eq ==> lalg_eq ==> lalg_eq) LABinop.
+    Proper (eq ==> lnra_eq ==> lnra_eq ==> lnra_eq) LNRABinop.
   Proof.
-    unfold Proper, respectful, lalg_eq; intros.
+    unfold Proper, respectful, lnra_eq; intros.
     subst.
     cbn.
     rewrite <- H0, H1 by trivial.
@@ -101,9 +101,9 @@ Section LambdaNRAEq.
   Qed.
 
   Global Instance launop_proper :
-    Proper (eq ==> lalg_eq ==> lalg_eq) LAUnop.
+    Proper (eq ==> lnra_eq ==> lnra_eq) LNRAUnop.
   Proof.
-    unfold Proper, respectful, lalg_eq; intros.
+    unfold Proper, respectful, lnra_eq; intros.
     subst.
     cbn.
     rewrite <- H0 by trivial.
@@ -111,72 +111,72 @@ Section LambdaNRAEq.
   Qed.
 
   Global Instance lamap_proper :
-    Proper (lalg_lambda_eq ==> lalg_eq ==> lalg_eq) LAMap.
+    Proper (lnra_lambda_eq ==> lnra_eq ==> lnra_eq) LNRAMap.
   Proof.
-    unfold Proper, respectful, lalg_eq, lalg_lambda_eq; intros.
-    autorewrite with lalg.
+    unfold Proper, respectful, lnra_eq, lnra_lambda_eq; intros.
+    autorewrite with lnra.
     rewrite <- H0 by trivial.
     apply olift_ext; intros.
     apply lift_oncoll_ext; intros; subst.
     f_equal.
     apply rmap_ext; intros.
     apply H; trivial.
-    eapply fun_of_lalg_normalized in H1; trivial.
+    eapply fun_of_lnra_normalized in H1; trivial.
     invcs H1.
     rewrite Forall_forall in H4.
     eauto.
   Qed.
 
   Global Instance lamapconcat_proper :
-    Proper (lalg_lambda_eq ==> lalg_eq ==> lalg_eq) LAMapConcat.
+    Proper (lnra_lambda_eq ==> lnra_eq ==> lnra_eq) LNRAMapConcat.
   Proof.
-    unfold Proper, respectful, lalg_eq, lalg_lambda_eq; intros.
-    autorewrite with lalg.
+    unfold Proper, respectful, lnra_eq, lnra_lambda_eq; intros.
+    autorewrite with lnra.
     rewrite <- H0 by trivial.
     apply olift_ext; intros.
     apply lift_oncoll_ext; intros; subst.
     f_equal.
     apply rmap_concat_ext; intros.
     apply H; trivial.
-    eapply fun_of_lalg_normalized in H1; trivial.
+    eapply fun_of_lnra_normalized in H1; trivial.
     invcs H1.
     rewrite Forall_forall in H4.
     eauto.
   Qed.
   
   Global Instance laproduct_proper :
-    Proper (lalg_eq ==> lalg_eq ==> lalg_eq) LAProduct.
+    Proper (lnra_eq ==> lnra_eq ==> lnra_eq) LNRAProduct.
   Proof.
-    unfold Proper, respectful, lalg_eq, lalg_lambda_eq; intros.
-    autorewrite with lalg.
+    unfold Proper, respectful, lnra_eq, lnra_lambda_eq; intros.
+    autorewrite with lnra.
     simpl.
     rewrite <- H, H0 by trivial.
     trivial.
   Qed.
 
-  Global Instance laselect_proper :
-    Proper (lalg_lambda_eq ==> lalg_eq ==> lalg_eq) LASelect.
+  Global Instance lafilter_proper :
+    Proper (lnra_lambda_eq ==> lnra_eq ==> lnra_eq) LNRAFilter.
   Proof.
-    unfold Proper, respectful, lalg_eq, lalg_lambda_eq; intros.
-    autorewrite with lalg.
+    unfold Proper, respectful, lnra_eq, lnra_lambda_eq; intros.
+    autorewrite with lnra.
     rewrite <- H0 by trivial.
     apply olift_ext; intros.
     apply lift_oncoll_ext; intros; subst.
     f_equal.
     apply lift_filter_ext; intros.
     rewrite H; trivial.
-    eapply fun_of_lalg_normalized in H1; trivial.
+    eapply fun_of_lnra_normalized in H1; trivial.
     invcs H1.
     rewrite Forall_forall in H4.
     eauto.
   Qed.
 
   Global Instance lalambda_proper :
-    Proper (eq ==> lalg_eq ==> lalg_lambda_eq) LALambda.
+    Proper (eq ==> lnra_eq ==> lnra_lambda_eq) LNRALambda.
   Proof.
-    unfold Proper, respectful, lalg_eq, lalg_lambda_eq; intros.
+    unfold Proper, respectful, lnra_eq, lnra_lambda_eq; intros.
     subst.
-    autorewrite with lalg.
+    autorewrite with lnra.
     rewrite H0.
     - reflexivity.
     - trivial.
