coq/Compiler/CompilerDriver/CompLang.v
@@ -52,7 +52,7 @@ Section CompLang.
   Definition camp := pat.
   Definition oql := oql.
   Definition sql := sql.
-  Definition lambda_nra := lalg.
+  Definition lambda_nra := lnra.
   Definition nra := alg.
   Definition nraenv_core := algenv.
   Definition nraenv := nraenv.
